@prefix bics: <https://github.com/tundrarich/tundrarich.github.io/blob/main/ontology/bics/> .
@prefix bics1: <https://github.com/tundrarich/tundrarich.github.io/blob/main/ontology/bics.ttl> .
@prefix dc: <http://purl.org/dc/elements/1.1/> .
@prefix owl: <http://www.w3.org/2002/07/owl#> .
@prefix rdf: <http://www.w3.org/1999/02/22-rdf-syntax-ns#> .
@prefix rdfs: <http://www.w3.org/2000/01/rdf-schema#> .
@prefix xsd: <http://www.w3.org/2001/XMLSchema#> .

bics:Industry a rdfs:Class ;
    rdfs:label "Industry" ;
    rdfs:comment "The class of an of Industry." ;
    rdfs:isDefinedBy bics: ;
    rdfs:subClassOf rdfs:Resource .

bics:Initiative a rdfs:Class ;
    rdfs:label "Initiative" ;
    rdfs:comment "The class of an Initiative." ;
    rdfs:isDefinedBy bics: ;
    rdfs:subClassOf rdfs:Resource .

bics:Location a rdfs:Class ;
    rdfs:label "Location" ;
    rdfs:comment "The class of a Location." ;
    rdfs:isDefinedBy bics: ;
    rdfs:subClassOf rdfs:Resource .

bics:Survey a rdfs:Class ;
    rdfs:label "Survey" ;
    rdfs:comment "The class of a Survey." ;
    rdfs:isDefinedBy bics: ;
    rdfs:subClassOf rdfs:Resource .

bics:TradingStatus a rdfs:Class ;
    rdfs:label "TradingStatus" ;
    rdfs:comment "The class of a Trading Status." ;
    rdfs:isDefinedBy bics: ;
    rdfs:subClassOf rdfs:Resource .

bics:WorkforceBand a rdfs:Class ;
    rdfs:label "WorkforceBand" ;
    rdfs:comment "The class of a certain workforce band size." ;
    rdfs:isDefinedBy bics: ;
    rdfs:subClassOf rdfs:Resource .

bics:ContainedIndustry a rdf:Property ;
    rdfs:label "ContainedIndustry" ;
    rdfs:comment "The property that refers to the Industry a resource can contain." ;
    rdfs:domain rdfs:Resource ;
    rdfs:isDefinedBy bics: ;
    rdfs:range rdfs:Resource .

bics:ContainedInitiative a rdf:Property ;
    rdfs:label "ContainedIniative" ;
    rdfs:comment "The property that refers to the Initiative a resource can contain." ;
    rdfs:domain rdfs:Resource ;
    rdfs:isDefinedBy bics: ;
    rdfs:range rdfs:Resource .

bics:ContainedLocation a rdf:Property ;
    rdfs:label "ContainedLocation" ;
    rdfs:comment "The property that refers to the Location a resource can contain." ;
    rdfs:domain rdfs:Resource ;
    rdfs:isDefinedBy bics: ;
    rdfs:range rdfs:Resource .

bics:ContainedTradingStatus a rdf:Property ;
    rdfs:label "ContainedTradingStatus" ;
    rdfs:comment "The property that refers to the TradingStatus a resource can contain." ;
    rdfs:domain rdfs:Resource ;
    rdfs:isDefinedBy bics: ;
    rdfs:range rdfs:Resource .

bics:ContainedWorkforce a rdf:Property ;
    rdfs:label "ContainedWorkforce" ;
    rdfs:comment "The property that refers to the workforceBand a resource can contain." ;
    rdfs:domain rdfs:Resource ;
    rdfs:isDefinedBy bics: ;
    rdfs:range rdfs:Resource .

bics:hasWorkforceNumberReceived a rdf:Property ;
    rdfs:label "hasWorkforceNumberReceived" ;
    rdfs:comment "The property that determines the number of workplaces that have a falls within a certain size-band surveys received numerically." ;
    rdfs:domain bics:WorkforceBand ;
    rdfs:isDefinedBy bics: ;
    rdfs:range rdfs:Resource .

bics:hasWorkforceNumberSent a rdf:Property ;
    rdfs:label "hasWorkforceNumberSent" ;
    rdfs:comment "The property that determines the number of workplaces that have a falls within a certain size-band surveys sent numerically." ;
    rdfs:domain bics:WorkforceBand ;
    rdfs:isDefinedBy bics: ;
    rdfs:range rdfs:Resource .

bics:hasWorkforcePercentageReceived a rdf:Property ;
    rdfs:label "WorkforcePercentageReceived" ;
    rdfs:comment "The property that determines the number of workplaces that have a falls within a certain size-band received percentage-wise." ;
    rdfs:domain bics:WorkforceBand ;
    rdfs:isDefinedBy bics: ;
    rdfs:range rdfs:Resource .

bics:initiativeStatus a rdf:Property ;
    rdfs:label "iniativeStatus" ;
    rdfs:comment "The property that determines the status of an Initiative." ;
    rdfs:domain bics:Initiative ;
    rdfs:isDefinedBy bics: ;
    rdfs:range rdfs:Resource .

bics:initiativeValue a rdf:Property ;
    rdfs:label "hasValue" ;
    rdfs:comment "The property that determines the value of the status a Initiative has." ;
    rdfs:domain bics:Initiative ;
    rdfs:isDefinedBy bics: ;
    rdfs:range rdfs:Resource .

bics:surveyDescription a rdf:Property ;
    rdfs:label "surveyDescription" ;
    rdfs:comment "The property that determines the description of the specific survey table." ;
    rdfs:domain bics:Survey ;
    rdfs:isDefinedBy bics: ;
    rdfs:range rdfs:Resource .

bics:tradingValue a rdf:Property ;
    rdfs:label "tradingValue" ;
    rdfs:comment "The property that determines the amount that is currently trading under a certain status." ;
    rdfs:domain bics:TradingStatus ;
    rdfs:isDefinedBy bics: ;
    rdfs:range rdfs:Resource .

<https://tundrarich.github.io/resources/survey/tradingStatusCountry> a bics1:Survey ;
    bics1:ContainedLocation <https://tundrarich.github.io/resources/locations/England>,
        <https://tundrarich.github.io/resources/locations/NorthernIreland>,
        <https://tundrarich.github.io/resources/locations/Scotland>,
        <https://tundrarich.github.io/resources/locations/UK>,
        <https://tundrarich.github.io/resources/locations/Wales> ;
    bics1:ContainedTradingStatus <https://tundrarich.github.io/resources/tradingStatuses/continuingTrading>,
        <https://tundrarich.github.io/resources/tradingStatuses/permanentlyCeasedTrading>,
        <https://tundrarich.github.io/resources/tradingStatuses/temporarilyClosedOrPausedTrading> ;
    bics1:surveyDescription "Question: What is the current trading status of your enterprise?, Percentage of all responding businesses, broken down by country, UK, 6 April to 19 April 2020"^^xsd:string .

<https://tundrarich.github.io/resources/tradingStatuses/continuingTrading/England> bics1:ContainedLocation <https://tundrarich.github.io/resources/locations/England> ;
    bics1:tradingValue "77.80%" .

<https://tundrarich.github.io/resources/tradingStatuses/continuingTrading/NorthernIreland> bics1:ContainedLocation <https://tundrarich.github.io/resources/locations/NorthernIreland> ;
    bics1:tradingValue "72.80%" .

<https://tundrarich.github.io/resources/tradingStatuses/continuingTrading/Scotland> bics1:ContainedLocation <https://tundrarich.github.io/resources/locations/Scotland> ;
    bics1:tradingValue "77.60%" .

<https://tundrarich.github.io/resources/tradingStatuses/continuingTrading/UK> bics1:ContainedLocation <https://tundrarich.github.io/resources/locations/UK> ;
    bics1:tradingValue "76.70%" .

<https://tundrarich.github.io/resources/tradingStatuses/continuingTrading/Wales> bics1:ContainedLocation <https://tundrarich.github.io/resources/locations/Wales> ;
    bics1:tradingValue "76.20%" .

<https://tundrarich.github.io/resources/tradingStatuses/permanentlyCeasedTrading/England> bics1:ContainedLocation <https://tundrarich.github.io/resources/locations/England> ;
    bics1:tradingValue "0.00%" .

<https://tundrarich.github.io/resources/tradingStatuses/permanentlyCeasedTrading/NorthernIreland> bics1:ContainedLocation <https://tundrarich.github.io/resources/locations/NorthernIreland> ;
    bics1:tradingValue "0.00%" .

<https://tundrarich.github.io/resources/tradingStatuses/permanentlyCeasedTrading/Scotland> bics1:ContainedLocation <https://tundrarich.github.io/resources/locations/Scotland> ;
    bics1:tradingValue "0.00%" .

<https://tundrarich.github.io/resources/tradingStatuses/permanentlyCeasedTrading/UK> bics1:ContainedLocation <https://tundrarich.github.io/resources/locations/UK> ;
    bics1:tradingValue "0.00%" .

<https://tundrarich.github.io/resources/tradingStatuses/permanentlyCeasedTrading/Wales> bics1:ContainedLocation <https://tundrarich.github.io/resources/locations/Wales> ;
    bics1:tradingValue "1.10%" .

<https://tundrarich.github.io/resources/tradingStatuses/temporarilyClosedOrPausedTrading/England> bics1:ContainedLocation <https://tundrarich.github.io/resources/locations/England> ;
    bics1:tradingValue "21.80%" .

<https://tundrarich.github.io/resources/tradingStatuses/temporarilyClosedOrPausedTrading/NorthernIreland> bics1:ContainedLocation <https://tundrarich.github.io/resources/locations/NorthernIreland> ;
    bics1:tradingValue "27.20%" .

<https://tundrarich.github.io/resources/tradingStatuses/temporarilyClosedOrPausedTrading/Scotland> bics1:ContainedLocation <https://tundrarich.github.io/resources/locations/Scotland> ;
    bics1:tradingValue "21.70%" .

<https://tundrarich.github.io/resources/tradingStatuses/temporarilyClosedOrPausedTrading/UK> bics1:ContainedLocation <https://tundrarich.github.io/resources/locations/UK> ;
    bics1:tradingValue "22.80%" .

<https://tundrarich.github.io/resources/tradingStatuses/temporarilyClosedOrPausedTrading/Wales> bics1:ContainedLocation <https://tundrarich.github.io/resources/locations/Wales> ;
    bics1:tradingValue "22.70%" .

<https://tundrarich.github.io/resources/tradingStatuses/continuingTrading> a bics1:TradingStatus ;
    rdfs:label "Continuing to trade"^^xsd:string .

<https://tundrarich.github.io/resources/locations/England> a bics1:Location ;
    rdfs:label "England"^^xsd:string ;
    bics1:ContainedTradingStatus <https://tundrarich.github.io/resources/tradingStatuses/continuingTrade>,
        <https://tundrarich.github.io/resources/tradingStatuses/permanentlyCeasedTrading>,
        <https://tundrarich.github.io/resources/tradingStatuses/temporarilyClosedOrPausedTrading> .

<https://tundrarich.github.io/resources/locations/NorthernIreland> a bics1:Location ;
    rdfs:label "Northern Ireland"^^xsd:string ;
    bics1:ContainedTradingStatus <https://tundrarich.github.io/resources/tradingStatuses/continuingTrade>,
        <https://tundrarich.github.io/resources/tradingStatuses/permanentlyCeasedTrading>,
        <https://tundrarich.github.io/resources/tradingStatuses/temporarilyClosedOrPausedTrading> .

<https://tundrarich.github.io/resources/locations/Scotland> a bics1:Location ;
    rdfs:label "Scotland"^^xsd:string ;
    bics1:ContainedTradingStatus <https://tundrarich.github.io/resources/tradingStatuses/continuingTrade>,
        <https://tundrarich.github.io/resources/tradingStatuses/permanentlyCeasedTrading>,
        <https://tundrarich.github.io/resources/tradingStatuses/temporarilyClosedOrPausedTrading> .

<https://tundrarich.github.io/resources/locations/UK> a bics1:Location ;
    rdfs:label "UK"^^xsd:string ;
    bics1:ContainedTradingStatus <https://tundrarich.github.io/resources/tradingStatuses/continuingTrade>,
        <https://tundrarich.github.io/resources/tradingStatuses/permanentlyCeasedTrading>,
        <https://tundrarich.github.io/resources/tradingStatuses/temporarilyClosedOrPausedTrading> .

<https://tundrarich.github.io/resources/locations/Wales> a bics1:Location ;
    rdfs:label "Wales"^^xsd:string ;
    bics1:ContainedTradingStatus <https://tundrarich.github.io/resources/tradingStatuses/continuingTrade>,
        <https://tundrarich.github.io/resources/tradingStatuses/permanentlyCeasedTrading>,
        <https://tundrarich.github.io/resources/tradingStatuses/temporarilyClosedOrPausedTrading> .

<https://tundrarich.github.io/resources/tradingStatuses/permanentlyCeasedTrading> a bics1:TradingStatus ;
    rdfs:label "Has permanently ceased trading"^^xsd:string .

<https://tundrarich.github.io/resources/tradingStatuses/temporarilyClosedOrPausedTrading> a bics1:TradingStatus ;
    rdfs:label "Has temporarily closed or temporarily paused trading"^^xsd:string .

bics: a owl:Ontology ;
    dc:date "2020-03-25" ;
    dc:description "BICS Vocabularly." ;
    dc:title "BICS Vocabularly" .

