@prefix bics: <https://github.com/tundrarich/tundrarich.github.io/blob/main/ontology/bics/> .
@prefix dc: <http://purl.org/dc/elements/1.1/> .
@prefix grddl: <http://www.w3.org/2003/g/data-view#> .
@prefix owl: <http://www.w3.org/2002/07/owl#> .
@prefix rdf: <http://www.w3.org/1999/02/22-rdf-syntax-ns#> .
@prefix rdfs: <http://www.w3.org/2000/01/rdf-schema#> .
@prefix xml: <http://www.w3.org/XML/1998/namespace> .
@prefix xsd: <http://www.w3.org/2001/XMLSchema#> .


<https://tundrarich.github.io/ontology/bics/> a owl:Ontology ;
	dc:title "BICS Vocabularly" ;
	dc:date "2020-03-25" ;
	dc:description "BICS Vocabularly." .
	owl:imports "https://github.com/tundrarich/tundrarich.github.io/blob/main/ontology/bics/" .

bics:Survey a rdfs:Class ;
     rdfs:label "Survey" ;
     rdfs:comment "The class of a Survey." ;
     rdfs:isDefinedBy <https://github.com/tundrarich/tundrarich.github.io/blob/main/ontology/bics/> ;
     rdfs:subClassOf rdfs:Resource . 

bics:Industry a rdfs:Class ;
     rdfs:label "Industry" ;
     rdfs:comment "The class of an of Industry." ;
     rdfs:isDefinedBy <https://github.com/tundrarich/tundrarich.github.io/blob/main/ontology/bics/> ;
     rdfs:subClassOf rdfs:Resource . 

bics:WorkforceBand a rdfs:Class ;
     rdfs:label "WorkforceBand" ;
     rdfs:comment "The class of a certain workforce band size." ;
     rdfs:isDefinedBy <https://github.com/tundrarich/tundrarich.github.io/blob/main/ontology/bics/> ;
     rdfs:subClassOf rdfs:Resource . 

bics:TradingStatus a rdfs:Class ;
     rdfs:label "TradingStatus" ;
     rdfs:comment "The class of a Trading Status." ;
     rdfs:isDefinedBy <https://github.com/tundrarich/tundrarich.github.io/blob/main/ontology/bics/> ;
     rdfs:subClassOf rdfs:Resource . 

bics:Location a rdfs:Class ;
     rdfs:label "Location" ;
     rdfs:comment "The class of a Location." ;
     rdfs:isDefinedBy <https://github.com/tundrarich/tundrarich.github.io/blob/main/ontology/bics/> ;
     rdfs:subClassOf rdfs:Resource . 

bics:Initiative a rdfs:Class ;
     rdfs:label "Initiative" ;
     rdfs:comment "The class of an Initiative." ;
     rdfs:isDefinedBy <https://github.com/tundrarich/tundrarich.github.io/blob/main/ontology/bics/> ;
     rdfs:subClassOf rdfs:Resource .

bics:ContainedIndustry a rdf:Property ;
     rdfs:label "ContainedIndustry" ;
     rdfs:comment "The property that refers to the Industry a resource can contain." ;
     rdfs:domain rdfs:Resource ;
     rdfs:isDefinedBy <https://github.com/tundrarich/tundrarich.github.io/blob/main/ontology/bics/> ;
     rdfs:range rdfs:Resource . 	 

bics:ContainedWorkforce a rdf:Property ;
     rdfs:label "ContainedWorkforce" ;
     rdfs:comment "The property that refers to the workforceBand a resource can contain." ;
     rdfs:domain rdfs:Resource ;
     rdfs:isDefinedBy <https://github.com/tundrarich/tundrarich.github.io/blob/main/ontology/bics/> ;
     rdfs:range rdfs:Resource . 

bics:ContainedLocation a rdf:Property ;
     rdfs:label "ContainedLocation" ;
     rdfs:comment "The property that refers to the Location a resource can contain." ;
     rdfs:domain rdfs:Resource ;
     rdfs:isDefinedBy <https://github.com/tundrarich/tundrarich.github.io/blob/main/ontology/bics/> ;
     rdfs:range rdfs:Resource .

bics:ContainedTradingStatus a rdf:Property ;
     rdfs:label "ContainedTradingStatus" ;
     rdfs:comment "The property that refers to the TradingStatus a resource can contain." ;
     rdfs:domain rdfs:Resource ;
     rdfs:isDefinedBy <https://github.com/tundrarich/tundrarich.github.io/blob/main/ontology/bics/> ;
     rdfs:range rdfs:Resource .
	 
bics:ContainedInitiative a rdf:Property ;
     rdfs:label "ContainedIniative" ;
     rdfs:comment "The property that refers to the Initiative a resource can contain." ;
     rdfs:domain rdfs:Resource ;
     rdfs:isDefinedBy <https://github.com/tundrarich/tundrarich.github.io/blob/main/ontology/bics/> ;
     rdfs:range rdfs:Resource .

bics:hasWorkforceNumberSent a rdf:Property ;
     rdfs:label "hasWorkforceNumberSent" ;
     rdfs:comment "The property that determines the number of workplaces that have a falls within a certain size-band surveys sent numerically." ;
     rdfs:domain bics:WorkforceBand ;
     rdfs:isDefinedBy <https://github.com/tundrarich/tundrarich.github.io/blob/main/ontology/bics/> ;
     rdfs:range rdfs:Resource . 

bics:hasWorkforceNumberReceived a rdf:Property ;
     rdfs:label "hasWorkforceNumberReceived" ;
     rdfs:comment "The property that determines the number of workplaces that have a falls within a certain size-band surveys received numerically." ;
     rdfs:domain bics:WorkforceBand ;
     rdfs:isDefinedBy <https://github.com/tundrarich/tundrarich.github.io/blob/main/ontology/bics/> ;
     rdfs:range rdfs:Resource . 
	  
bics:hasWorkforcePercentageReceived a rdf:Property ;
     rdfs:label "WorkforcePercentageReceived" ;
     rdfs:comment "The property that determines the number of workplaces that have a falls within a certain size-band received percentage-wise." ;
     rdfs:domain bics:WorkforceBand ;
     rdfs:isDefinedBy <https://github.com/tundrarich/tundrarich.github.io/blob/main/ontology/bics/> ;
     rdfs:range rdfs:Resource . 

	 
bics:tradingValue a rdf:Property ;
     rdfs:label "tradingValue" ;
     rdfs:comment "The property that determines the amount that is currently trading under a certain status." ;
     rdfs:domain bics:TradingStatus ;
     rdfs:isDefinedBy <https://github.com/tundrarich/tundrarich.github.io/blob/main/ontology/bics/> ;
     rdfs:range rdfs:Resource . 
	 
bics:initiativeStatus a rdf:Property ;
     rdfs:label "iniativeStatus" ;
     rdfs:comment "The property that determines the status of an Initiative." ;
     rdfs:domain bics:Initiative ;
     rdfs:isDefinedBy <https://github.com/tundrarich/tundrarich.github.io/blob/main/ontology/bics/> ;
     rdfs:range rdfs:Resource . 

bics:initiativeValue a rdf:Property ;
     rdfs:label "hasValue" ;
     rdfs:comment "The property that determines the value of the status a Initiative has." ;
     rdfs:domain bics:Initiative ;
     rdfs:isDefinedBy <https://github.com/tundrarich/tundrarich.github.io/blob/main/ontology/bics/> ;
     rdfs:range rdfs:Resource . 

bics:surveyDescription a rdf:Property ;
     rdfs:label "surveyDescription" ;
     rdfs:comment "The property that determines the description of the specific survey table." ;
     rdfs:domain bics:Survey ;
     rdfs:isDefinedBy <https://github.com/tundrarich/tundrarich.github.io/blob/main/ontology/bics/> ;
     rdfs:range rdfs:Resource . 
	 
	 
	 





